add actions and prove some invariants

PBFT.thy
@@ -7,38 +7,188 @@ definition compatible where
 
 statespace ('p, 'v, 'b) vars =
   committed :: "'p \<Rightarrow> 'v::linorder \<Rightarrow> 'b::order \<Rightarrow> bool"
-  commit_msg :: "'p \<Rightarrow>  'v::linorder \<Rightarrow> 'b::order \<Rightarrow> bool"
+  prepared :: "'p \<Rightarrow>  'v \<Rightarrow> 'b \<Rightarrow> bool"
+  pre_prepared :: "'p \<Rightarrow> 'v \<Rightarrow> 'b \<Rightarrow> bool"
+  view :: "'p \<Rightarrow> 'v"
 
 no_notation Set.member  (\<open>'(\<in>')\<close>)
 no_notation Set.member  (\<open>(\<open>notation=\<open>infix \<in>\<close>\<close>_/ \<in> _)\<close> [51, 51] 50)
 
-locale pbft = vars _ _ project_HOL_bool_'b_fun_'v_fun_'p_fun
+print_locale vars
+
+locale pbft = vars _ _ _ _ _ _ project_HOL_bool_'b_fun_'v_fun_'p_fun
   for  project_HOL_bool_'b_fun_'v_fun_'p_fun :: "_ \<Rightarrow> 'p \<Rightarrow> 'v::linorder \<Rightarrow> 'b::order \<Rightarrow> bool" + \<comment> \<open>boilerplate to unify type variables\<close>
   fixes quorum_member :: "'p \<Rightarrow> 'q \<Rightarrow> bool" (infix "\<in>" 50)
     and byz :: "'p \<Rightarrow> bool"
   assumes "\<And> q1 q2 . \<exists> p . \<not> byz p \<and> p \<in> q1 \<and> p \<in> q2" \<comment> \<open>quorum intersection\<close>
 begin
 
+definition inv0 where
+  \<comment> \<open>No correct party has pre-prepared, prepared, or committed anything after its current view\<close>
+  "inv0 s \<equiv> undefined"
+
 definition inv1 where
-  "inv1 s \<equiv> \<forall> p v b . \<not> byz p \<and> (s\<cdot>committed) p v b \<longrightarrow> (\<exists> q . \<forall> p' . p' \<in> q \<and> \<not> byz p' \<longrightarrow> (s\<cdot>commit_msg) p' v b)"
+  \<comment> \<open>If a party commits a block, then a quorum has prepared it\<close>
+  "inv1 s \<equiv> \<forall> p v b . \<not> byz p \<and> (s\<cdot>committed) p v b \<longrightarrow> (\<exists> q . \<forall> p' . p' \<in> q \<and> \<not> byz p' \<longrightarrow> (s\<cdot>prepared) p' v b)"
 
 definition inv2 where
-  "inv2 s \<equiv> \<forall> p v b . \<not> byz p \<and> (s\<cdot>commit_msg) p v b \<longrightarrow> (\<forall> p' v' b' . \<not> byz p' \<and> v' < v \<and> (s\<cdot>committed) p' v' b' \<longrightarrow> b' \<le> b)"
+  \<comment> \<open>If a party prepares a block, then a quorum has pre-prepared it\<close>
+  "inv2 s \<equiv> \<forall> p v b . \<not> byz p \<and> (s\<cdot>prepared) p v b \<longrightarrow> (\<exists> q . \<forall> p' . p' \<in> q \<and> \<not> byz p' \<longrightarrow> (s\<cdot>pre_prepared) p' v b)"
 
 definition inv3 where
-  "inv3 s \<equiv> \<forall> p p' v b b' . \<not> byz p \<and> \<not> byz p' \<and> (s\<cdot>commit_msg) p v b \<and> (s\<cdot>commit_msg) p' v b' \<longrightarrow> b = b'"
+  \<comment> \<open>No honest party pre-prepares two different blocks in the same view\<close>
+  "inv3 s \<equiv> \<forall> p v b b' . \<not> byz p \<and> (s\<cdot>pre_prepared) p v b \<and> (s\<cdot>pre_prepared) p v b' \<longrightarrow> b = b'"
+
+definition safe where
+  \<comment> \<open>A block b is safe in view v when no block that is incompatible or longer can be committed in any previous view\<close>
+  "safe s b v \<equiv> (\<forall> p' v' b' . \<not> byz p' \<and> v' < v \<and> (s\<cdot>committed) p' v' b' \<longrightarrow> b' \<le> b)"
+
+definition inv4 where
+  \<comment> \<open>If a party pre-prepares a block b in view v, then b is safe in v\<close>
+  "inv4 s \<equiv> \<forall> p v b . \<not> byz p \<and> (s\<cdot>pre_prepared) p v b \<longrightarrow> safe s b v"
+
+section \<open>Specification of the algorithm\<close>
+
+definition init where
+  "init s \<equiv> \<forall> p v b .
+      \<not>(s\<cdot>committed) p v b
+    \<and> \<not>(s\<cdot>prepared) p v b
+    \<and> \<not>(s\<cdot>pre_prepared) p v b"
+
+definition commit where
+  "commit s s' p q v b \<equiv>
+      \<not> byz p
+    \<and> (v = (s\<cdot>view) p)
+    \<and> (\<forall> p' . p' \<in> q \<and> \<not> byz p' \<longrightarrow> (s\<cdot>prepared) p' v b)
+    \<and> s' = s<committed := (s\<cdot>committed)(p := ((s\<cdot>committed) p)(v := ((s\<cdot>committed) p v)(b := True)))>"
+
+definition prepare where
+  "prepare s s' p q v b \<equiv>
+      \<not> byz p
+    \<and> (v = (s\<cdot>view) p)
+    \<and> (\<forall> p' . p' \<in> q \<and> \<not> byz p' \<longrightarrow> (s\<cdot>pre_prepared) p' v b)
+    \<and> s' = s<prepared := (s\<cdot>prepared)(p := ((s\<cdot>prepared) p)(v := ((s\<cdot>prepared) p v)(b := True)))>"
+
+definition pre_prepare where
+  \<comment> \<open>pre-prepare a safe block\<close>
+  "pre_prepare s s' p v b \<equiv> undefined"
+
+definition change_view where
+  \<comment> \<open>Start a higher view\<close>
+  "change_view s s' p v \<equiv> undefined"
+
+definition trans_rel where
+  "trans_rel s s' p q v b \<equiv>
+      commit s s' p q v b
+    \<or> prepare s s' p q v b"
+
+section \<open>Induction proofs\<close>
+
+lemma inv1_inductive:
+  shows "init s \<Longrightarrow> inv1 s" and "trans_rel s s' p q v b \<and> inv1 s \<Longrightarrow> inv1 s'"
+proof -
+  show "init s \<Longrightarrow> inv1 s"
+    by (simp add: init_def inv1_def)
+next
+  show "trans_rel s s' p q v b \<and> inv1 s \<Longrightarrow> inv1 s'"
+    unfolding trans_rel_def commit_def prepare_def inv1_def
+    apply auto
+        apply (smt (verit) fun_upd_apply)
+       apply meson+
+    done
+qed
+
+lemma inv2_inductive:
+  shows "init s \<Longrightarrow> inv2 s" and "trans_rel s s' p q v b \<and> inv2 s \<Longrightarrow> inv2 s'"
+proof -
+  show "init s \<Longrightarrow> inv2 s"
+    by (simp add: init_def inv2_def)
+next
+  show "trans_rel s s' p q v b \<and> inv2 s \<Longrightarrow> inv2 s'"
+    unfolding trans_rel_def
+    apply (auto; simp add: commit_def prepare_def inv2_def; auto)
+    done
+qed
+
+lemma inv3_inductive:
+  shows "init s \<Longrightarrow> inv3 s" and "trans_rel s s' p q v b \<and> inv3 s \<Longrightarrow> inv3 s'"
+proof -
+  show "init s \<Longrightarrow> inv3 s"
+    by (simp add: init_def inv3_def)
+next
+  show "trans_rel s s' p q v b \<and> inv3 s \<Longrightarrow> inv3 s'"
+    unfolding trans_rel_def
+    apply (auto; simp add: commit_def prepare_def inv3_def; auto)
+    done
+qed
+
+lemma inv4_inductive:
+  shows "init s \<Longrightarrow> inv4 s" and "trans_rel s s' p q v b \<and> inv4 s \<Longrightarrow> inv4 s'"
+proof -
+  show "init s \<Longrightarrow> inv4 s"
+    by (simp add: init_def inv4_def safe_def)
+next
+  show "trans_rel s s' p q v b \<and> inv4 s \<Longrightarrow> inv4 s'"
+  proof -
+    assume asm: "trans_rel s s' p q v b \<and> inv4 s"
+    then have "commit s s' p q v b \<or> prepare s s' p q v b"
+      unfolding trans_rel_def by simp
+    then show "inv4 s'"
+    proof
+      assume "commit s s' p q v b"
+      \<comment> \<open>Case 1: commit transition - show inv4 s'\<close>
+      \<comment> \<open>Key idea: pre_prepared is unchanged by commit, so anything pre-prepared in s' was already pre-prepared in s\<close>
+      show ?thesis
+        sorry
+    next
+      assume "prepare s s' p q v b"
+      \<comment> \<open>Case 2: prepare transition - show inv4 s'\<close>
+      \<comment> \<open>Key idea: pre_prepared is unchanged by prepare, so anything pre-prepared in s' was already pre-prepared in s\<close>
+      show ?thesis
+        using \<open>prepare s s' p q v b\<close> asm inv4_def prepare_def safe_def by auto
+    qed
+  qed
+  oops
+
+lemma l0:
+  fixes s p p' v b b'
+  assumes "inv2 s" and "inv3 s" 
+    and "\<not> byz p" and "\<not>byz p'" 
+    and "(s\<cdot>prepared) p v b" and "(s\<cdot>prepared) p' v b'"
+  shows "b = b'"
+proof -
+  \<comment> \<open>From p's prepared message, a quorum pre-prepared b\<close>
+  obtain q1 where q1: "\<forall> p1 . p1 \<in> q1 \<and> \<not> byz p1 \<longrightarrow> (s\<cdot>pre_prepared) p1 v b"
+    using assms(1,3,5) unfolding inv2_def by blast
+  
+  \<comment> \<open>From p''s prepared message, a quorum pre-prepared b'\<close>
+  obtain q2 where q2: "\<forall> p2 . p2 \<in> q2 \<and> \<not> byz p2 \<longrightarrow> (s\<cdot>pre_prepared) p2 v b'"
+    using assms(1,4,6) unfolding inv2_def by blast
+  
+  \<comment> \<open>By quorum intersection, there's an honest party in both quorums\<close>
+  obtain p'' where p'': "\<not> byz p''" "p'' \<in> q1" "p'' \<in> q2"
+    using pbft_axioms unfolding pbft_def pbft_axioms_def by blast
+  
+  \<comment> \<open>This party pre-prepared both b and b'\<close>
+  have "(s\<cdot>pre_prepared) p'' v b" using q1 p'' by blast
+  moreover have "(s\<cdot>pre_prepared) p'' v b'" using q2 p'' by blast
+  
+  \<comment> \<open>By inv3, they must be equal\<close>
+  ultimately show "b = b'"
+    using assms(2) p''(1) unfolding inv3_def by blast
+qed
 
 lemma l1:
   fixes s p v b p' v' b'
-  assumes "inv1 s" and "inv2 s" and "inv3 s" and "\<not> byz p" and "\<not> byz p'"
+  assumes "inv1 s" and "inv2 s" and "inv3 s" and "inv4 s" and "\<not> byz p" and "\<not> byz p'"
     and "(s\<cdot>committed) p v b" and "(s\<cdot>committed) p' v' b'"
   shows "compatible b b'"
 proof -
-  \<comment> \<open>Obtain non-Byzantine processes that sent commit messages\<close>
-  obtain p1 where p1: "\<not> byz p1" "(s\<cdot>commit_msg) p1 v b"
-    using assms(1,4,6) pbft_axioms unfolding inv1_def pbft_def pbft_axioms_def by blast
-  obtain p2 where p2: "\<not> byz p2" "(s\<cdot>commit_msg) p2 v' b'"
+  \<comment> \<open>Obtain non-Byzantine processes that prepared the blocks\<close>
+  obtain p1 where p1: "\<not> byz p1" "(s\<cdot>prepared) p1 v b"
     using assms(1,5,7) pbft_axioms unfolding inv1_def pbft_def pbft_axioms_def by blast
+  obtain p2 where p2: "\<not> byz p2" "(s\<cdot>prepared) p2 v' b'"
+    using assms(1,6,8) pbft_axioms unfolding inv1_def pbft_def pbft_axioms_def by blast
   
   \<comment> \<open>Case analysis on the relationship between v and v'\<close>
   consider (less) "v < v'" | (equal) "v = v'" | (greater) "v' < v"
@@ -46,21 +196,35 @@ proof -
   then show ?thesis
   proof cases
     case less
-    \<comment> \<open>v < v': use inv2 with p2's commit_msg and p's commitment\<close>
-    from p2(1) p2(2) assms(4) less assms(6) have "b \<le> b'"
-      using assms(2) unfolding inv2_def by blast
+    \<comment> \<open>v < v': need to show b \<le> b' using safety\<close>
+    \<comment> \<open>From p2's prepared message, obtain a quorum that pre-prepared b'\<close>
+    obtain q where q: "\<forall> p'' . p'' \<in> q \<and> \<not> byz p'' \<longrightarrow> (s\<cdot>pre_prepared) p'' v' b'"
+      using assms(2) p2 unfolding inv2_def by blast
+    \<comment> \<open>By quorum intersection, there's an honest party in q\<close>
+    obtain p'' where p'': "\<not> byz p''" "p'' \<in> q"
+      using pbft_axioms unfolding pbft_def pbft_axioms_def by metis
+    \<comment> \<open>This party pre-prepared b' at v', so by inv4, b' is safe at v'\<close>
+    have "(s\<cdot>pre_prepared) p'' v' b'" using q p'' by blast
+    then have "safe s b' v'" using assms(4) p''(1) unfolding inv4_def by blast
+    \<comment> \<open>Since v < v' and p committed b at v, we have b \<le> b'\<close>
+    then have "b \<le> b'" using less assms(5,7) unfolding safe_def by blast
     thus ?thesis unfolding compatible_def by auto
   next
     case equal
-    \<comment> \<open>v = v': use inv3 to show b = b'\<close>
+    \<comment> \<open>v = v': use l0 to show b = b'\<close>
     from p1 p2 equal have "b = b'"
-      using assms(3) unfolding inv3_def by blast
+      using l0[OF assms(2,3) p1(1) p2(1)] by simp
     thus ?thesis unfolding compatible_def by auto
   next
     case greater
-    \<comment> \<open>v' < v: use inv2 with p1's commit_msg and p''s commitment\<close>
-    from p1(1) p1(2) assms(5) greater assms(7) have "b' \<le> b"
-      using assms(2) unfolding inv2_def by blast
+    \<comment> \<open>v' < v: symmetric to the less case\<close>
+    obtain q where q: "\<forall> p'' . p'' \<in> q \<and> \<not> byz p'' \<longrightarrow> (s\<cdot>pre_prepared) p'' v b"
+      using assms(2) p1 unfolding inv2_def by blast
+    obtain p'' where p'': "\<not> byz p''" "p'' \<in> q"
+      using pbft_axioms unfolding pbft_def pbft_axioms_def by metis
+    have "(s\<cdot>pre_prepared) p'' v b" using q p'' by blast
+    then have "safe s b v" using assms(4) p''(1) unfolding inv4_def by blast
+    then have "b' \<le> b" using greater assms(6,8) unfolding safe_def by blast
     thus ?thesis unfolding compatible_def by auto
   qed
 qed
